src/impl/TLS13.Impl.Server.Setup.fsti
@@ -98,6 +98,49 @@ fn process_select_server_parameters
                    network_out_bytes
                    app_out_bytes)
 
+fn process_select_server_parameters_with_private_from_array
+  (s:server)
+  (server_private_key:array U8.t)
+  (#selection:erased CS.server_handshake_selection)
+  (network_out:array U8.t)
+  (network_out_len:SZ.t)
+  (app_out:array U8.t)
+  (app_out_len:SZ.t)
+  requires connection_exactly s 'st0 **
+           pts_to server_private_key 'server_private_key_bytes **
+           pts_to network_out 'old_network_out **
+           pts_to app_out 'old_app_out **
+           pure (B.length 'server_private_key_bytes == 32 /\
+                  B.length 'old_network_out == SZ.v network_out_len /\
+                  B.length 'old_app_out == SZ.v app_out_len /\
+                  ST.server_end_to_end_invariant 'st0 /\
+                  CM.can_select_server_parameters 'st0 selection /\
+                  CR.server_selection_absent
+                    'st0.CS.cs_model.CS.model_handshake /\
+                  Some? selection.CS.server_key_share_private /\
+                  Some?.v selection.CS.server_key_share_private ==
+                    Ghost.reveal 'server_private_key_bytes)
+  returns resp:ST.server_response
+  ensures exists* st1 network_out_bytes app_out_bytes.
+          connection_exactly s st1 **
+          pts_to server_private_key 'server_private_key_bytes **
+          pts_to network_out network_out_bytes **
+          pts_to app_out app_out_bytes **
+          pure (B.length network_out_bytes == SZ.v network_out_len /\
+                B.length app_out_bytes == SZ.v app_out_len /\
+                st1 ==
+                  CM.selected_server_parameters_state
+                    'st0
+                    (Ghost.reveal selection) /\
+                ST.server_local_event_end_to_end_correct
+                   'st0
+                   st1
+                   resp
+                   ST.LocalSelectServerParameters
+                   B.empty
+                   network_out_bytes
+                   app_out_bytes)
+
 fn process_select_default_server_parameters_from_arrays
   (s:server)
   (server_random:array U8.t)
@@ -164,6 +207,89 @@ fn process_select_default_server_parameters_from_arrays
                         cfg.CS.server_credential_identity;
                     } in
                     st1 == CM.selected_server_parameters_state 'st0 selection
+                  | _ -> True)) /\
+                ST.server_local_event_end_to_end_correct
+                  'st0
+                  st1
+                  resp
+                  ST.LocalSelectServerParameters
+                  B.empty
+                  network_out_bytes
+                  app_out_bytes)
+
+fn process_select_default_server_parameters_with_private_from_arrays
+  (s:server)
+  (server_random:array U8.t)
+  (server_private_key:array U8.t)
+  (server_key_share:array U8.t)
+  (network_out:array U8.t)
+  (network_out_len:SZ.t)
+  (app_out:array U8.t)
+  (app_out_len:SZ.t)
+  requires connection_exactly s 'st0 **
+           pts_to server_random 'server_random_bytes **
+           pts_to server_private_key 'server_private_key_bytes **
+           pts_to server_key_share 'server_key_share_bytes **
+           pts_to network_out 'old_network_out **
+           pts_to app_out 'old_app_out **
+           pure (B.length 'server_random_bytes == 32 /\
+                 B.length 'server_private_key_bytes == 32 /\
+                 B.length 'server_key_share_bytes == 32 /\
+                 B.length 'old_network_out == SZ.v network_out_len /\
+                 B.length 'old_app_out == SZ.v app_out_len /\
+                 ST.server_end_to_end_invariant 'st0 /\
+                 CR.server_selection_absent
+                  'st0.CS.cs_model.CS.model_handshake /\
+                 Some? 'st0.CS.cs_model.CS.model_handshake.CS.hs_client_hello /\
+                 Some? 'st0.CS.cs_model.CS.model_config.CS.config_server /\
+                 (let ch =
+                   Some?.v 'st0.CS.cs_model.CS.model_handshake.CS.hs_client_hello in
+                  let cfg =
+                   Some?.v 'st0.CS.cs_model.CS.model_config.CS.config_server in
+                  let selection = {
+                   CS.server_selected_client_hello = ch;
+                   CS.server_selected_cipher_suite =
+                     T.TLS_CHACHA20_POLY1305_SHA256;
+                   CS.server_selected_group = T.X25519;
+                   CS.server_selected_signature_scheme = T.RsaPssRsaeSha256;
+                   CS.server_random = Ghost.reveal 'server_random_bytes;
+                   CS.server_key_share_private =
+                     Some (Ghost.reveal 'server_private_key_bytes);
+                   CS.server_key_share_public = Ghost.reveal 'server_key_share_bytes;
+                   CS.server_selected_credential =
+                     cfg.CS.server_credential_identity;
+                  } in
+                  CM.can_select_server_parameters 'st0 selection))
+  returns resp:ST.server_response
+  ensures exists* st1 network_out_bytes app_out_bytes.
+          connection_exactly s st1 **
+          pts_to server_random 'server_random_bytes **
+          pts_to server_private_key 'server_private_key_bytes **
+          pts_to server_key_share 'server_key_share_bytes **
+          pts_to network_out network_out_bytes **
+          pts_to app_out app_out_bytes **
+          pure (B.length network_out_bytes == SZ.v network_out_len /\
+                B.length app_out_bytes == SZ.v app_out_len /\
+                (B.length (Ghost.reveal 'server_random_bytes) == 32 /\
+                 B.length (Ghost.reveal 'server_private_key_bytes) == 32 /\
+                 B.length (Ghost.reveal 'server_key_share_bytes) == 32 ==>
+                 (match 'st0.CS.cs_model.CS.model_handshake.CS.hs_client_hello,
+                       'st0.CS.cs_model.CS.model_config.CS.config_server with
+                  | Some ch, Some cfg ->
+                   let selection = {
+                     CS.server_selected_client_hello = ch;
+                     CS.server_selected_cipher_suite =
+                       T.TLS_CHACHA20_POLY1305_SHA256;
+                     CS.server_selected_group = T.X25519;
+                     CS.server_selected_signature_scheme = T.RsaPssRsaeSha256;
+                     CS.server_random = Ghost.reveal 'server_random_bytes;
+                     CS.server_key_share_private =
+                       Some (Ghost.reveal 'server_private_key_bytes);
+                     CS.server_key_share_public = Ghost.reveal 'server_key_share_bytes;
+                     CS.server_selected_credential =
+                       cfg.CS.server_credential_identity;
+                   } in
+                   st1 == CM.selected_server_parameters_state 'st0 selection
                   | _ -> True)) /\
                 ST.server_local_event_end_to_end_correct
                   'st0
